generalise wp-diffpriv and -sensitivity to distances instead of |x-y|%Z

theories/diffpriv/examples/diffpriv_basic_examples.v
@@ -1,3 +1,4 @@
+From clutch.common Require Import inject.
 From clutch.prob Require Import differential_privacy.
 From clutch.diffpriv Require Import adequacy diffpriv proofmode.
 
@@ -20,105 +21,6 @@ Section wp_example.
     tp_bind (Laplace _ _ _).
     iApply (wp_couple_laplace _ _ 0%Z with "[$]") => //.
     setoid_rewrite Z.add_0_r. done.
-  Qed.
-
-  Definition wp_sensitive (f : expr) (c : R) := ∀ (c_pos : 0 <= c) K (x x' : Z),
-    {{{ ⤇ fill K (f #x') }}}
-      f #x
-      {{{ (v : Z), RET #v; ∃ v' : Z, ⤇ fill K (Val #v') ∧ ⌜IZR (Z.abs (v - v')) <= c * IZR (Z.abs (x - x'))⌝ }}}.
-
-  Definition wp_diffpriv (f : expr) ε := ∀ K c (x x' : Z), IZR (Z.abs (x - x')) <= c →
-      {{{ ⤇ fill K (f #x') ∗ ↯ (c * ε) }}} f #x {{{ (z : Z), RET #z; ⤇ fill K (Val #z) }}}.
-
-  Fact wp_lap_dipr (num den : Z) :
-    0 < IZR num / IZR den →
-    wp_diffpriv (λ: "loc", Laplace #num #den "loc")%E ((IZR num / IZR den)).
-  Proof.
-    intros. rewrite /wp_diffpriv. intros K c x x' adj.
-    iIntros (φ) "[f' ε] hφ".
-    opose proof (wp_laplace_diffpriv x x' num den _ _) as h => //. simpl in h.
-    iPoseProof (h φ with "[f' ε]") as "h".
-    { iFrame. iApply ec_weaken. 2: iFrame.
-      split. 1: rewrite abs_IZR ; real_solver_partial. 1: apply Rabs_pos. 1: lra.
-      apply Rmult_le_compat => //. 1: rewrite abs_IZR ; apply Rabs_pos. lra.
-    }
-    iApply "h". done.
-  Qed.
-
-  Fact sensitive_comp (g f : val) cg cf (cg_pos : 0 <= cg) (cf_pos : 0 <= cf) :
-    wp_sensitive g cg → wp_sensitive f cf → wp_sensitive (λ:"x", g (f "x")) (cg * cf).
-  Proof.
-    rewrite /wp_sensitive. intros g_sens f_sens. intros. iIntros "f' hΦ".
-    wp_pures. wp_bind (f _). tp_pures. tp_bind (f _).
-    iApply (f_sens with "[$f']") => //.
-    iIntros "!>" (fx) "(%fx' & gv' & %sens)".
-    iApply (g_sens with "[$gv']") => //.
-    iIntros "!>" (gfx) "(%gfx'' & vv' & %sens')".
-    iApply "hΦ". iExists _. iFrame. iPureIntro.
-    etrans => //.
-    rewrite Rmult_assoc.
-    eapply Rmult_le_compat_l => //.
-  Qed.
-
-  Fact diffpriv_diffpriv_comp (g f : val) εg εf (εg_pos : 0 <= εg) (εf_pos : 0 <= εf) :
-    wp_diffpriv g εg → wp_diffpriv f εf → wp_diffpriv (λ:"x", g (f "x")) εf.
-  Proof.
-    rewrite /wp_sensitive/wp_diffpriv. intros g_dipr f_dipr. intros. iIntros "[gf' εf] hΦ".
-    wp_pures. wp_bind (f _). tp_pures. tp_bind (f _).
-    iApply (f_dipr with "[$gf' $εf]") => //. iNext. iIntros (?) "g'".
-    iPoseProof (g_dipr K 0 z z) as "g_dipr".
-    { rewrite !abs_IZR. replace (z-z)%Z with 0%Z by lia. rewrite Rabs_R0. done. }
-    iMod ec_zero as "ε0".
-    replace (0 * εg) with 0 by lra.
-    iApply ("g_dipr" with "[$ε0 $g']"). done.
-  Qed.
-
-  Fact diffpriv_sensitive_comp (g f : val) ε c (c_pos : 0 <= c) : wp_diffpriv g ε → wp_sensitive f c → wp_diffpriv (λ:"x", g (f "x")) (c*ε).
-  Proof.
-    rewrite /wp_sensitive/wp_diffpriv. intros g_dipr f_sens. intros K c'. intros. iIntros "[f' ε] hΦ".
-    wp_pures. wp_bind (f _). tp_pures. tp_bind (f _).
-    iApply (f_sens with "[$f']") => //.
-    iIntros "!>" (?) "(%v' & gv' & %sens)".
-    iPoseProof (g_dipr K (c * c')) as "g_dipr".
-    { etrans => //. apply Rmult_le_compat_l => //. }
-    iApply ("g_dipr" with "[$gv' ε]") => //. rewrite (Rmult_comm c) Rmult_assoc. done.
-  Qed.
-
-  Definition wp_fun (f : expr) := ∀ K (v : Z),
-    {{{ ⤇ fill K (f #v) }}}
-      f #v
-      {{{ (x : Z), RET #x; ⤇ fill K (Val #x) }}}.
-
-  Fact refl_diffpriv_comp (g f : val) ε c (c_pos : 0 <= c)
-    : wp_diffpriv g ε → wp_fun f → wp_diffpriv (λ:"x", f (g "x")) ε.
-  Proof.
-    rewrite /wp_sensitive/wp_diffpriv. intros g_dipr f_sens. intros K c' ?? adj ?. intros. iIntros "[g ε] hΦ".
-    wp_pures. wp_bind (g _). tp_pures. tp_bind (g _).
-    iApply (g_dipr _ c' with "[$g ε]") => //.
-    iNext. iIntros (?) "f'".
-    iApply (f_sens with "[$f']").
-    iIntros "!>" (?) "gv'".
-    iApply "hΦ". done.
-  Qed.
-
-  Fact sens_refl (f : val) c (c_pos : 0 <= c) : wp_sensitive f c → wp_fun f.
-  Proof.
-    iIntros (f_sens K z Φ) "f' hΦ".
-    iApply (f_sens c_pos K z z with "f'").
-    iNext. iIntros (v) "(%v' & v' & %sens)".
-    iApply "hΦ".
-    assert (v = v') as -> => //.
-    move: sens. rewrite !abs_IZR. replace (z-z)%Z with 0%Z by lia. rewrite Rabs_R0.
-    pose proof (Rabs_pos (IZR (v - v'))) as h. intros. assert (Rabs (IZR (v - v')) = 0) as h' by lra.
-    rewrite -abs_IZR in h'. revert h'. apply Zabs_ind.
-    - intros. assert (v - v' = 0)%Z by apply eq_IZR =>//. lia.
-    - intros. assert (- (v - v') = 0)%Z by apply eq_IZR =>//. lia.
-  Qed.
-
-  Corollary sensitive_diffpriv_comp (g f : val) ε c (c_pos : 0 <= c)
-    : wp_diffpriv g ε → wp_sensitive f c → wp_diffpriv (λ:"x", f (g "x")) ε.
-  Proof.
-    intros. eapply refl_diffpriv_comp => //. eapply sens_refl => //.
   Qed.
 
   Definition ID := Fst.
@@ -183,7 +85,7 @@ Fact Laplace_diffpriv σ (num den : Z) :
     ε.
 Proof.
   intros ε εpos.
-  eapply (adequacy.wp_diffpriv diffprivΣ) ; eauto ; try lra.
+  eapply (adequacy.wp_diffpriv_Z diffprivΣ) ; eauto ; try lra.
   iIntros (????) "f' ε".
   iApply (wp_laplace_diffpriv _ _ _ _ [] with "[f' ε]") => //.
   2: eauto.
@@ -192,21 +94,4 @@ Proof.
   split.
   - apply Rmult_le_pos. 2: subst ε ; lra. apply IZR_le. lia.
   - etrans. 2: right ; apply Rmult_1_l. apply Rmult_le_compat_r. 1: lra. done.
-Qed.
-
-(* wp_diffpriv implies pure diffpriv *)
-Fact wp_diffpriv_pure f ε (εpos : (0 < ε)%R) :
-  (∀ `{diffprivGS Σ}, wp_diffpriv f ε)
-  →
-    ∀ σ,
-    diffpriv_pure
-      (λ x y, IZR (Z.abs (x - y)))
-      (λ x, lim_exec (f #x, σ))
-      ε.
-Proof.
-  intros hwp ?.
-  eapply (adequacy.wp_diffpriv diffprivΣ) ; eauto ; try lra.
-  iIntros (????) "f' ε".
-  iApply (hwp _ _ [] 1%R with "[$f' ε]") => //. 1: rewrite Rmult_1_l ; done.
-  iNext. iIntros. iExists _. eauto.
 Qed.
